More work towards lazy int refining eager

theories/examples/lazy_int.v
@@ -47,6 +47,24 @@ Section lazy_int.
         else
           "res".
 
+  Definition sample_lazy_int : val :=
+    λ: "_",
+      let: "hd" := ref NONEV in
+      let: "α" := alloc in
+      ("α", "hd").
+
+  Definition sample_eager_int : val :=
+    λ: "_",
+      let: "α" := alloc in
+      sample_wide_int PRED_NUM_CHUNKS PRED_CHUNK_BITS ("α").
+
+  Definition cmp_lazy_int : val :=
+    λ: "lz1" "lz2",
+      cmp_list #NUM_CHUNKS (Fst "lz1" )(Snd "lz1") (Fst "lz2" )(Snd "lz2").
+
+  Definition cmp_eager_int : val :=
+    cmpZ.
+
   Context `{!prelogrelGS Σ}.
 
   Fixpoint chunk_list l (zs : list Z) : iProp Σ :=
@@ -127,6 +145,24 @@ Section lazy_int.
       wp_pures. iApply "HΦ"; eauto.
   Qed.
 
+  Lemma spec_cmpZ (z1 z2 : Z) E K :
+    ↑specN ⊆ E →
+    refines_right K (cmpZ #z1 #z2) ={E}=∗
+    refines_right K (of_val #(comparison2z (Z.compare z1 z2))).
+  Proof.
+    iIntros (?) "HK".
+    rewrite /cmpZ.
+    destruct (Z.compare_spec z1 z2).
+    - tp_pures K; case_bool_decide; try lia.
+      tp_pures K; case_bool_decide; try lia.
+      tp_pures K. by iFrame.
+    - tp_pures K; case_bool_decide; try lia.
+      tp_pures K. by iFrame.
+    - tp_pures K; case_bool_decide; try lia.
+      tp_pures K; case_bool_decide; try lia.
+      tp_pures K. by iFrame.
+  Qed.
+
   Lemma wp_cmp_list n α1 α2 l1 l2 zs1 zs2 E :
     n = length zs1 →
     n = length zs2 →
@@ -172,6 +208,86 @@ Section lazy_int.
         iPureIntro. simpl. destruct (z1 ?= z2)%Z; try eauto.
         simpl in Hcase; congruence.
       }
+  Qed.
+
+  Definition lazy_int (z: Z) (v: val) : iProp Σ :=
+    ∃ (α l : loc) zs, ⌜ v = (#lbl:α, #l)%V ⌝ ∗
+                      ⌜ z = digit_list_to_Z PRED_CHUNK_BITS zs ⌝ ∗
+                      ⌜ length zs = NUM_CHUNKS ⌝ ∗
+                      ⌜ wf_digit_list PRED_CHUNK_BITS zs ⌝ ∗
+                      chunk_and_tape_list α l zs.
+
+  Lemma wp_sample_lazy_eager_couple K E :
+    ↑ specN ⊆ E →
+    {{{ refines_right K (sample_eager_int #()) }}}
+      sample_lazy_int #() @ E
+    {{{ v, RET v; ∃ z, lazy_int z v ∗ refines_right K (of_val #z) }}}.
+  Proof.
+    iIntros (? Φ) "HK HΦ".
+    rewrite /sample_lazy_int.
+    wp_pures.
+    wp_alloc l as "Hl".
+    wp_pures.
+    wp_apply (wp_alloc_tape with "[//]").
+    iIntros (α) "Hα".
+
+    rewrite /sample_eager_int.
+    tp_pures K.
+    tp_alloctape K as αₛ "Hαₛ".
+    tp_pures K.
+    iApply (wp_couple_int_tapesN_eq PRED_CHUNK_BITS _ _ NUM_CHUNKS).
+    { eauto. }
+    { eauto. }
+    iSplit.
+    { iDestruct "HK" as "($&_)". }
+    iSplitL "Hαₛ".
+    { iApply spec_int_tape_intro. iFrame. }
+    iSplitL "Hα".
+    { iApply int_tape_intro. iFrame. }
+    iDestruct 1 as (zs Hrange Hlegnth) "(Hspec_tape&Htape)".
+    iMod (spec_sample_wide_int _ _ _ _ _ _ [] with "[Hspec_tape] [$]") as (z) "(HK&%Hz&_)"; auto.
+    { eauto. }
+    { rewrite app_nil_l app_nil_r. iFrame. }
+    wp_pures. iApply "HΦ". iExists _. iFrame.
+    iModIntro. iExists _, _, _.
+    iSplit; first eauto.
+    iSplit; first eauto.
+    iSplit; first eauto.
+    iSplit.
+    { iPureIntro. rewrite /wf_digit_list. eapply Forall_impl; try eassumption.
+      intros x => /=. rewrite /MAX_INT Z.ones_equiv/NUM_BITS.
+      lia. }
+    iExists [], zs.
+    rewrite app_nil_l. iFrame.
+    eauto.
+  Qed.
+
+  Lemma wp_cmp_lazy_eager_refine z1 z2 v1 v2 K E :
+    ↑ specN ⊆ E →
+    {{{ lazy_int z1 v1 ∗ lazy_int z2 v2 ∗ refines_right K (cmp_eager_int #z1 #z2) }}}
+      cmp_lazy_int v1 v2 @ E
+    {{{ zret, RET #zret ;
+        ⌜ zret = (comparison2z (Z.compare z1 z2)) ⌝ ∗
+        lazy_int z1 v1 ∗ lazy_int z2 v2 ∗ refines_right K (of_val #zret) }}}.
+  Proof.
+    iIntros (HE Φ) "(Hv1&Hv2&HK) HΦ".
+    iDestruct "Hv1" as (α1 l1 zs1 -> Hz1 Hlen1 Hwf1) "H1".
+    iDestruct "Hv2" as (α2 l2 zs2 -> Hz2 Hlen2 Hwf2) "H2".
+    rewrite /cmp_lazy_int. wp_pures.
+    iApply wp_fupd.
+    wp_apply (wp_cmp_list with "[$H1 $H2]"); try done.
+    iIntros (zret) "(%Hret&H1&H2)".
+    iMod (spec_cmpZ with "[$]") as "HK"; first done.
+    iModIntro. iApply "HΦ".
+    assert (zret = comparison2z (z1 ?= z2)%Z) as Hreteq.
+    { rewrite Hret. f_equal.
+      rewrite Hz1 Hz2.
+      eapply digit_list_cmp_spec; eauto.
+      lia. }
+    iSplit; first eauto. rewrite Hreteq. iFrame.
+    iSplitL "H1".
+    { iExists _, _, _. iFrame. eauto. }
+    { iExists _, _, _. iFrame. eauto. }
   Qed.
 
 End lazy_int.
